add zippers in racket mode and make the big oh proof nicer

clrs/from_zip_gen.rkt
@@ -1,0 +1,8 @@
+#lang at-exp s-exp tmonad
+(provide from_zip)
+
+(Fixpoint
+ from_zip
+ @A{Set} @z{Zipper A} @ALL_RIGHT{(fst z) = nil}
+ #:returns @{list A}
+ (<== (snd z)))
