clrs/insert_at_gen.rkt
@@ -1,0 +1,16 @@
+#lang at-exp s-exp tmonad
+(provide insert_at)
+
+(Fixpoint
+ insert_at
+ @A{Set} @a{A} @n{nat} @l{list A} @NV{n <= length l}
+ #:returns @{list A}
+ (match (n)
+   [O =>
+    (<== (cons a l))]
+   [(S np) =>
+    (match (l)
+      [(nil) => (<== _)]
+      [(cons ap lp) =>
+       (bind ([resp (insert_at A a np lp _)])
+             (<== (cons ap resp)))])]))
