clrs/minsert_at_gen.rkt
@@ -1,0 +1,14 @@
+#lang at-exp s-exp tmonad
+(require "insert_at_gen.rkt")
+(provide minsert_at)
+
+(Fixpoint
+ minsert_at
+ @A{Set} @ma{list A} @n{nat} @l{list A} @NV{n <= length l}
+ #:returns @{list A}
+ (match (ma)
+   [(nil) => (<== l)]
+   [(cons a map) =>
+    (bind ([resp (insert_at A a n l NV)])
+          (bind ([respp (minsert_at A map n resp _)])
+                (<== respp)))]))
