clrs/minsertz_at_gen.rkt
@@ -1,0 +1,18 @@
+#lang at-exp s-exp tmonad
+(require "to_zip_gen.rkt"
+         "zip_rightn_gen.rkt"
+         "zip_minsert_gen.rkt"
+         "zip_leftn_gen.rkt"
+         "from_zip_gen.rkt")
+(provide minsertz_at)
+
+(Fixpoint
+ minsertz_at
+ @A{Set} @ma{list A} @n{nat} @l{list A} @NV{n <= length l}
+ #:returns @{list A}
+ (bind ([z (to_zip A l)])
+       (bind ([zr (zip_rightn A n z _)])
+             (bind ([zrp (zip_minsert A ma zr)])
+                   (bind ([zp (zip_leftn A n zrp _)])
+                         (bind ([lp (from_zip A zp _)])
+                               (<== lp)))))))
