clrs/to_zip_gen.rkt
@@ -1,0 +1,8 @@
+#lang at-exp s-exp tmonad
+(provide to_zip)
+
+(Fixpoint
+ to_zip
+ @A{Set} @l{list A}
+ #:returns @{Zipper A}
+ (<== (pair nil l)))
