clrs/zip_insert_gen.rkt
@@ -1,0 +1,8 @@
+#lang at-exp s-exp tmonad
+(provide zip_insert)
+
+(Fixpoint
+ zip_insert
+ @A{Set} @z{Zipper A} @a{A}
+ #:returns @{Zipper A}
+ (<== (pair (fst z) (cons a (snd z)))))
