clrs/zip_left_gen.rkt
@@ -1,0 +1,11 @@
+#lang at-exp s-exp tmonad
+(provide zip_left)
+
+(Fixpoint
+ zip_left
+ @A{Set} @z{Zipper A} @SOME_LEFT{(fst z) <> nil}
+ #:returns @{Zipper A}
+ (match ((fst z))
+   [(nil) => (<== _)]
+   [(cons b xs) =>
+    (<== (pair xs (cons b (snd z))))]))
