clrs/zip_leftn_gen.rkt
@@ -1,0 +1,14 @@
+#lang at-exp s-exp tmonad
+(require "zip_left_gen.rkt")
+(provide zip_leftn)
+
+(Fixpoint
+ zip_leftn
+ @A{Set} @n{nat} @z{Zipper A} @NV{n <= length (fst z)}
+ #:returns @{Zipper A}
+ (match (n)
+   [O => (<== z)]
+   [(S np) =>
+    (bind ([zp (zip_left A z _)])
+          (bind ([zpp (zip_leftn A np zp _)])
+                (<== zpp)))]))
