clrs/zip_minsert_gen.rkt
@@ -1,0 +1,14 @@
+#lang at-exp s-exp tmonad
+(require "zip_insert_gen.rkt")
+(provide zip_minsert)
+
+(Fixpoint
+ zip_minsert
+ @A{Set} @ma{list A} @z{Zipper A}
+ #:returns @{Zipper A}
+ (match (ma)
+   [(nil) => (<== z)]
+   [(cons a map) =>
+    (bind ([zp (zip_insert A z a)])
+          (bind ([zpp (zip_minsert A map zp)])
+                (<== zpp)))]))
