clrs/zip_right_gen.rkt
@@ -1,0 +1,11 @@
+#lang at-exp s-exp tmonad
+(provide zip_right)
+
+(Fixpoint
+ zip_right
+ @A{Set} @z{Zipper A} @SOME_RIGHT{(snd z) <> nil}
+ #:returns @{Zipper A}
+ (match ((snd z))
+   [(nil) => (<== _)]
+   [(cons a ys) =>
+    (<== (pair (cons a (fst z)) ys))]))
