clrs/zip_rightn_gen.rkt
@@ -1,0 +1,14 @@
+#lang at-exp s-exp tmonad
+(require "zip_right_gen.rkt")
+(provide zip_rightn)
+
+(Fixpoint
+ zip_rightn
+ @A{Set} @n{nat} @z{Zipper A} @NV{n <= length (snd z)}
+ #:returns @{Zipper A}
+ (match (n)
+   [O => (<== z)]
+   [(S np) =>
+    (bind ([zp (zip_right A z _)])
+          (bind ([zpp (zip_rightn A np zp _)])
+                (<== zpp)))]))
