paper/line-counts.rkt
@@ -58,7 +58,11 @@
       "fib_rec_gen.v"))
     ("size"
      ("size_linear.v" "size_linear_gen.v")
-     ("size_log_sq.v" "diff_gen.v" "size_log_sq_gen.v"))))
+     ("size_log_sq.v" "diff_gen.v" "size_log_sq_gen.v"))
+    ("clrs"
+     ("zip.v" "from_zip_gen.v" "minsert_at_gen.v" "minsertz_at_gen.v"
+      "to_zip_gen.v" "zip_insert_gen.v" "zip_left_gen.v" "zip_leftn_gen.v"
+      "zip_minsert_gen.v" "zip_right_gen.v" "zip_rightn_gen.v"))))
 
 (define (build-table)
   (tabular
